\section{Elliptic Curve Arithmetic}
\label{section:ec}
\textbf{WIP}

\subsection{Incomplete Addition}

\begin{center}
    \begin{table}[H]
        \begin{tabular}{llllllllllllllll}
            Row   & 0     & 1     & 2     & 3     & 4     & 5     & 6   & 7       & 8       & 9       & 10      & 11      & 12      & 13      & 14      \\
            $i$ & $x_1$ & $y_1$ & $x_2$ & $y_2$ & $x_3$ & $y_3$ & $r$ & $\dots$ & $\dots$ & $\dots$ & $\dots$ & $\dots$ & $\dots$ & $\dots$ & $\dots$ \\
        \end{tabular}
    \end{table}
\end{center}

Constraints:
\begin{itemize}
    \item $(x_2 - x_1) \cdot (y_3 + y_1) - (y_1 - y_2) \cdot (x_1 - x_3) = 0$
    \item $(x_1 + x_2 + x_3) \cdot (x_1 - x_3) \cdot (x_1 - x_3) - (y_3 + y_1) \cdot (y_3 + y_1) = 0$
    \item $(x_2 - x_1) \cdot r = 1$
\end{itemize}

\subsection{Doubling and Tripling}

\begin{center}
    \begin{table}[H]
        \begin{tabular}{llllllllllllllll}
            Row   & 0     & 1     & 2     & 3     & 4     & 5     & 6     & 7     & 8       & 9       & 10      & 11      & 12      & 13      & 14      \\
            $i$ & $x_1$ & $y_1$ & $x_2$ & $y_2$ & $x_3$ & $y_3$ & $r_1$ & $r_2$ & $\dots$ & $\dots$ & $\dots$ & $\dots$ & $\dots$ & $\dots$ & $\dots$ \\
        \end{tabular}
    \end{table}
\end{center}

Constraints:
\begin{itemize}
    \item Doubling:
    \begin{itemize}
        \item $4 \cdot y_1^2 \cdot (x_2 + 2 \cdot x_1) = 9 \cdot x_1^4$
        \item $2 \cdot y_1 \cdot (y_2 + y_1) = (3 \cdot x_1^2) \cdot (x_1 - x_2)$
        \item $y_1 \cdot r_1 = 1$
    \end{itemize}
    \item Addition (for tripling):
    \begin{itemize}
        \item $(x_2 - x_1) \cdot (y_3 + y_1) - (y_1 - y_2) \cdot (x_1 - x_3) = 0$
        \item $(x_1 + x_2 + x_3) \cdot (x_1 - x_3) \cdot (x_1 - x_3) - (y_3 + y_1) \cdot (y_3 + y_1) = 0$
        \item $(x_2 - x_1) \cdot r_2 = 1$
    \end{itemize}
\end{itemize}

\subsection{Unified Incomplete Addition and Squaring}

\begin{center}
    \begin{table}[H]
        \begin{tabular}{llllllllllllllll}
            Row   & 0     & 1     & 2     & 3     & 4     & 5     & 6   & 7       & 8       & 9       & 10      & 11      & 12      & 13      & 14      \\
            $i$ & $x_1$ & $y_1$ & $x_2$ & $y_2$ & $x_3$ & $y_3$ & $\texttt{inf}$ & $\texttt{same\_x}$ & $s$ & $\texttt{inv}_y$ & $\texttt{inv}_x$ & $\dots$ & $\dots$ & $\dots$ & $\dots$ \\
        \end{tabular}
    \end{table}
\end{center}

Constraints ($\textbf{max degree} = 3$):
\begin{enumerate}
	 \item $w_7 \cdot (w_2 - w_0) = 0$
    \item $(w_2 - w_0) \cdot w_{10} - (1 - w_7) = 0$
    \item $w_7 \cdot (2w_8 \cdot w_1 - 3w_0^2) + (1 - w_7) \cdot (w_2 - w_0 \cdot w_8 - (w_3 - w_1))$
    \item $w_8^2 = w_0 + w_2 + w_4$
    \item $w_5 = w_8 \cdot (w_0 - w_4) - w_1$
    \item $(w_3 - w_1) \cdot (w_7 - w_6) = 0$
    \item $(w_3 - w_1) \cdot w_9 - w_6 = 0$
\end{enumerate}

\paragraph{Details.}

The gate uses basic group law formulae. 
Let $P = (x_1, y_1), Q = (x_2, y_2), R = (x_3, y_3)$ and $R = P + Q$. Then: 
\begin{itemize}
    \item $(x_2 - x_1) \cdot s = y_2 - y_1$
    \item $s^2 = x_1 + x_2 + x_3$
    \item $y_3 = s \cdot (x_1 - x_3) - y_1$
\end{itemize}
For point doubling $R = P + P = 2P$:
\begin{itemize}
    \item $2s \cdot y_1 = 3x_1^2$
    \item $s^2 = 2x_1 + x_3$
    \item $y_3 = s \cdot (x_1 - x_3) - y_1$
\end{itemize}

\begin{itemize}
	 \item $x_2 - x_1$ zero check:
	 \begin{enumerate}
		 	\item $w_7 \cdot (w_2 - w_0) = 0 \longleftrightarrow 
		 			\texttt{same\_x} \cdot (x_2 -x_1)$ \\
		 		If $x_1 \neq x_2$, then $\texttt{same\_x} = 0$
		    \item $(w_2 - w_0) \cdot w_{10} - (1 - w_7) = 0 \longleftrightarrow 
		    		(x_2 - x_1) \cdot \texttt{inv}_x - (1 - \texttt{same\_x})$ \\
		    	If $x_1 \neq x_2$, then $\texttt{inv}_x = (x_2 - x_1)^{-1}$
	 \end{enumerate}
	 \item Group law constraints:
	 \begin{enumerate}
	 	\item $w_7 \cdot (2w_8 \cdot w_1 - 3w_0^2) + (1 - w_7) \cdot ((w_2 - w_0 \cdot w_8 - (w_3 - w_1)) \longleftrightarrow$ \\
			  $\texttt{same\_x} \cdot (2s \cdot y_1 - 3x_1^2) + (1 - \texttt{same\_x}) \cdot (x_2 - x_1 \cdot s - (y_2 - y_1))$ \\
			If $x_1 = x_2$ then use doubling $2s \cdot y_1 = 3x_1^2$. Otherwise use addition $(x_2 - x_1) \cdot s = y_2 - y_1$.
	 	\item $w_8^2 = w_0 + w_2 + w_4 \longleftrightarrow 
	 			s^2 = x_1 + x_2 + x_3$ \\
	 		Constrains $x_3$. It does not depend on $x_1, x_2$ equality.
	 	\item $w_5 = w_8 \cdot (w_0 - w_4) - w_1 \longleftrightarrow 
	 			y_3 = s \cdot (x_1 - x_3) - y_1$ \\
	 		Constrains $y_3$. It does not depend on $x_1, x_2$ equality.
	 \end{enumerate}
	 \item $P + (-P)$ constraints:
	 \begin{enumerate}
		 \item $(w_3 - w_1) \cdot (w_7 - w_6) = 0 \longleftrightarrow 
	    			(y_2 - y_1) \cdot (\texttt{same\_x} - \texttt{inf}) = 0$ \\ 
	    	We can get inifinity point iff $x_1 = x_2$ and $y_1 \neq y_2$. \\
	    	If $y_1 \neq y_2$ then $\texttt{inf} = \texttt{same\_x}$.
	    \item $(w_3 - w_1) \cdot w_9 - w_6 = 0 \longleftrightarrow 
	    			(y_2 - y_1) \cdot \texttt{inv}_y - \texttt{inf}$ \\
	    	The prover sets $\texttt{inv}_y = 0$ for $y_1 = y_2$. \\
	    	If $y_1 \neq y_2$ then $\texttt{inv}_y = (y_2 - y_1)^{-1}$
	 \end{enumerate}
\end{itemize}

\subsection{Variable Base Scalar Multiplication}
For $S  = [r]T$, where $r = 2^n + k$ and $k = [k_n ... k_0]$, $k_i \in \{0, 1\}$:
\footnote{Using the results from \url{https://arxiv.org/pdf/math/0208038.pdf}}
\begin{enumerate}
    \item $S = [2]T$
    \item for $i$ from $n - 1$ to $0$:
    \begin{enumerate}
        \item $Q = k_{i + 1} \: ? \: T : -T$
        \item $R = S + Q$
        \item $S = R + S$
    \end{enumerate}
    \item $S = k_0 \: ? \: S - T : S$
\end{enumerate}

\begin{center}
    \begin{table}[H]
        \begin{tabular}{llllllllllllllll}
            Row     & 0        & 1        & 2        & 3        & 4        & 5        & 6        & 7        & 8        & 9        & 10       & 11       & 12       & 13       & 14       \\
            $i$    & $x_T$    & $y_T$    & $x_S$    & $y_S$    & $x_P$    & $y_P$    & $n=0$    & $x_R$    & $y_R$    & $s_1$    & $s_2$    & $b_1$    & $s_3$ & $s_4$ & $b_2$ \\
            $i + 1$   & $s_5$    & $b_3$    & $x_S$    & $y_S$    & $x_P$    & $y_P$    & $n$      & $x_R$    & $y_R$    & $x_V$    & $y_V$    & $s_1$    & $b_1$ & $s_3$ & $b_2$ \\
            $\vdots$  & $\vdots$ & $\vdots$ & $\vdots$ & $\vdots$ & $\vdots$ & $\vdots$ & $\vdots$ & $\vdots$ & $\vdots$ & $\vdots$ & $\vdots$ & $\vdots$ & $\vdots$ & $\vdots$ & $\vdots$ \\
            $i + 100$ & $x_T$    & $y_T$    & $x_S$    & $y_S$    & $x_P$    & $y_P$    & $n$      & $x_R$    & $y_R$    & $s_1$    & $s_2$    & $b_1$ & $s_3$ & $s_4$ & $b_2$ \\
            $i + 101$ & $s_5$    & $b_3$    & $x_S$    & $y_S$    & $x_P$    & $y_P$    & $n$      & $x_R$    & $y_R$    & $x_V$    & $y_V$    & $s_1$ & $b_1$ & $s_3$ & $b_2$ \\
        \end{tabular}
    \end{table}
\end{center}

Constraints for $i + z$, where $z\mod 2 = 0$:
\begin{itemize}
    \item $b_1 \cdot (b_1 - 1) = 0$
    \item $b_2 \cdot (b_2 - 1) = 0$
    \item $(x_P - x_T) \cdot s_1 = y_P - (2b_1 - 1) \cdot y_T$
    \item $s_1^2 - s_2^2 = x_T - x_R$
    \item $(2 \cdot x_P + x_T - s_1^2) \cdot (s_1 + s_2) = 2y_P$
    \item $(x_P - x_R) \cdot s_2 = y_R + y_P$
    \item $(x_R - x_T) \cdot s_3 = y_R - (2b_2 - 1) \cdot y_T$
    \item $s_3^2 - s_4^2 = x_T - x_S$
    \item $(2 \cdot x_R + x_T - s_3^2) \cdot (s_3 + s_4) = 2 \cdot y_R$
    \item $(x_R - x_S) \cdot s_4 = y_S + y_R$
    \item $n = 32 \cdot \texttt{next}(n) + 16 \cdot b_1 + 8 \cdot b_2 + 4 \cdot \texttt{next}(b_1) + 2 \cdot \texttt{next}(b_2) + \texttt{next}(b_3)$
\end{itemize}

Constraints for $i + z$, where $z\mod 2 = 1$:
\begin{itemize}
    \item $b_1 \cdot (b_1 - 1) = 0$
    \item $b_2 \cdot (b_2 - 1) = 0$
    \item $b_3 \cdot (b_3 - 1) = 0$
    \item $(x_P - x_T) \cdot s_1 = y_P - (2b_1 - 1) \cdot y_T$
    \item $(2 \cdot x_P + x_T - s_1^2) \cdot ((x_P - x_R) \cdot s_1 + y_R + y_P) = (x_P - x_R) \cdot 2y_P$\
    \item $(y_R + y_P)^2 = (x_P - x_R)^2 \cdot (s_1^2 - x_T + x_R)$
    \item $(x_T - x_R) \cdot s_3 = (2b_2 - 1) \cdot y_T - y_R$
    \item $(2x_R - s_3^2 + x_T) \cdot ((x_R - x_V) \cdot s_3 + y_V + y_R) = (x_R - x_V) \cdot 2y_R$
    \item $(y_V + y_R)^2 = (x_R - x_V)^2 \cdot (s_3^2 - x_T + x_V)$
    \item $(x_T - x_V) \cdot s_5 = (2b_3 - 1) \cdot y_T - y_V$
    \item $(2x_V - s_5^2 + x_T) \cdot ((x_V - x_S) \cdot s_5 + y_S + y_V) = (x_V - x_S) \cdot 2y_V$
    \item $(y_S + y_V)^2 = (x_V - x_S)^2 \cdot (s_5^2 - x_T + x_S)$
\end{itemize}

\subsection{Variable Base Endo-Scalar Multiplication}

For $S  = [r]T$, where $r = [r_n ... r_0]$ and $r_i \in \{0, 1\}$:
\footnote{Using the results from \url{https://eprint.iacr.org/2019/1021.pdf}}
\begin{enumerate}
    \item $S = [2](\phi(T) + T)$
    \item for $i$ from $\frac{\lambda}{2} - 1$ to $0$:
    \begin{enumerate}
        \item $Q = r_{2i + 1} \: ? \: \phi([2r_{2i} - 1]T) : [2r_{2i} - 1]T$
        \item $R = S + Q$
        \item $S = R + S$
    \end{enumerate}
\end{enumerate}

\begin{center}
    \begin{table}[H]
        \begin{tabular}{llllllllllllllll}
            Row    & 0        & 1        & 2        & 3        & 4        & 5        & 6        & 7        & 8        & 9        & 10       & 11       & 12       & 13       & 14       \\
            $i$   & $x_T$    & $y_T$    & $x_S$    & $y_S$    & $x_P$    & $y_P$    & $n$      & $x_R$    & $y_R$    & $s_1$    & $s_3$    & $b_1$    & $b_2$ & $b_3$ & $b_4$ \\
            $\vdots$ & $\vdots$ & $\vdots$ & $\vdots$ & $\vdots$ & $\vdots$ & $\vdots$ & $\vdots$ & $\vdots$ & $\vdots$ & $\vdots$ & $\vdots$ & $\vdots$ & $\vdots$ & $\vdots$ & $\vdots$ \\
            $i + 63$ &  $x_T$    & $y_T$    & $x_S$    & $y_S$    & $x_P$    & $y_P$    & $n$      & $x_R$    & $y_R$    & $s_1$    & $s_3$    & $b_1$    & $b_2$ & $b_3$ & $b_4$ \\
        \end{tabular}
    \end{table}
\end{center}

Constraints:
\begin{itemize}
    \item $b_1 \cdot (b_1 - 1) = 0$
    \item $b_2 \cdot (b_2 - 1) = 0$
    \item $b_3 \cdot (b_3 - 1) = 0$
    \item $b_4 \cdot (b_4 - 1) = 0$
    \item $((1 + (\texttt{endo} - 1) \cdot b_2) \cdot x_T - x_P) \cdot s_1 = (2 \cdot b_1 - 1) \cdot y_T - y_P$
    \item $(2 \cdot x_P - s_1^2 + (1 + (\texttt{endo} - 1) \cdot b_2) \cdot x_T) \cdot ((x_P - x_R) \cdot s_1 + y_R + y_P) = (x_P - x_R) \cdot 2 \cdot y_P$
    \item $(y_R + yP)^2 = (xP - x_R)^2 \cdot (s_1^2 - (1 + (\texttt{endo} - 1) \cdot b_2) \cdot x_T + x_R)$
    \item $((1 + (\texttt{endo} - 1) \cdot b_2) \cdot x_T - x_R) \cdot s_3 = (2 \cdot b_3-1) \cdot y_T - y_R$
    \item $(2 \cdot x_R - s_3^2 + (1 + (\texttt{endo} - 1) \cdot b_4) \cdot x_T) \cdot ((x_R - x_S) \cdot s_3 + y_S + y_R) = (x_R - x_S) \cdot 2 \cdot y_R$
    \item $(y_S + y_R)^2 = (x_R - x_S)^2 \cdot (s_3^2 - (1 + (\texttt{endo} - 1) \cdot b_4) \cdot x_T + x_S)$
    \item $n = 16 \cdot \texttt{next}(n) + 8 \cdot b_1 + 4 \cdot b_2 + 2 \cdot b_3 + b_4$
\end{itemize}

\subsection{Fixed-base scalar multiplication circuit}
We precompute all values $w(B,s,k) = (k_i + 2) \cdot 8^s B$, where $k_i \in \{ 0,..7 \}$, $s \in \{0,.., 83\}$ and  $w(B,s,k) = (k_i \cdot 8^s - \sum_{j = 0}^{84} 8^{j + 1}) \cdot B$, where $k_i \in \{ 0,..7 \}$, $s = 84$.
\begin{center}
    \begin{table}[H]
        \begin{tabular}{llllllllllllllll}
            Row        & 0        & 1        & 2        & 3        & 4        & 5        & 6        & 7        & 8        & 9        & 10       & 11        & 12       & 13       & 14       \\
            $i$      & $b_0$    & $b_1$    & $b_2$    & $b_3$    & $b_4$    & $b_5$    & $u_0$    & $u_1$    & $v_0$    & $v_1$    & $x_1$    & $y_1$     & $x_2$ & $y_2$ & $acc$ \\
            $\vdots$  & $\vdots$ & $\vdots$ & $\vdots$ & $\vdots$ & $\vdots$ & $\vdots$ & $\vdots$ & $\vdots$ & $\vdots$ & $\vdots$ & $\vdots$ & $\vdots$ & $\vdots$ & $\vdots$ & $\vdots$ \\
            $i + 42$ & $b_0$    & $b_1$    & $b_2$    & $u_0$    & $v_0$    & $x_w$    & $y_w$    & $\alpha$ & $\beta$  & $\gamma$ & $\delta$ & $\lambda$ & $-$ & $-$ & $b$ \\
        \end{tabular}
    \end{table}
\end{center}

Define the following functions:
\begin{enumerate}
    \item $\phi_1: (x_1, x_2, x_3, x_4) \mapsto $ \\
    $x_3 \cdot (-u'_0 \cdot x_2 \cdot x_1 + u'_0 \cdot x_1 + u'_0 \cdot x_2
    - u'_0 + u'_2 \cdot x_1 \cdot x_2 - u'_2\cdot x_2 + u'_4 \cdot x_1 \cdot x_2
    - u'_4\cdot x_2 -u'_6 \cdot x_1 \cdot x_2 + u'_1 \cdot x_2 \cdot x_1
    - u'_1 \cdot x_1 - u'_1 \cdot x_2 + u'_1  - u'_3 \cdot x_1 \cdot x_2 + u'_3\cdot x_2
    - u'_5 \cdot x_1 \cdot x_2 + u'_5\cdot x_2 + u'_7 \cdot x_1 \cdot x_2) -
    (x_4 - u'_0 \cdot x_2 \cdot x_1 + u'_0 \cdot x_1 + u'_0 \cdot x_2
    - u'_0 + u'_2 \cdot x_1 \cdot x_2 - u'_2\cdot x_2 + u'_4 \cdot x_1 \cdot x_2
    - u'_4\cdot x_2 -u'_6 \cdot x_1 \cdot x_2)$
    \item $\phi_2: (x_1, x_2, x_3, x_4) \mapsto $ \\
    $x_3 \cdot (-v'_0 \cdot x_2 \cdot x_1 + v'_0 \cdot x_1 + v'_0 \cdot x_2
    - v'_0 + v'_2 \cdot x_1 \cdot x_2 -v'_2 \cdot x_2 + v'_4 \cdot x_1 \cdot x_2
    - v'_4 \cdot x_2 - v'_6 \cdot x_1 \cdot x_2 + v'_1 \cdot x_2 \cdot x_1
    - v'_1 \cdot x_1 - v'_1 \cdot x_2 + v'_1  - v'_3 \cdot x_1 \cdot x_2
    + v'_3 \cdot x_2 - v'_5 \cdot x_1 \cdot x_2 + v'_5 \cdot x_2
    + v'_7 \cdot x_1 \cdot x_2) - (x_4 - v'_0 \cdot x_2 \cdot x_1
    + v'_0 \cdot x_1 + v'_0 \cdot x_2 - v'_0 + v'_2 \cdot x_1 \cdot x_2
    - v'_2 \cdot x_2 + v'_4 \cdot x_1 \cdot x_2 - v'_4 \cdot x_2 - v'_6 \cdot x_1 \cdot x_2) $
\end{enumerate}

Constraints:
\begin{itemize}
    \item For $i + 0$:
    \begin{itemize}
        \item $b_i \cdot (b_i - 1) = 0$, where $i \in\{0,.., 5\}$
        \item $\phi_1(b_0, b_1, b_2, u_0) = 0$, where $(u'_{i}, v'_{i}) = w(B, 0, i)$
        \item $\phi_1(b_3, b_4, b_5, u_1) = 0$, where $(u'_{i}, v'_{i}) = w(B, 1, i)$
        \item $\phi_2(b_0, b_1, b_2, v_0) = 0$, where $(u'_{i}, v'_{i}) = w(B, 0, i)$
        \item $\phi_2(b_3, b_4, b_5, v_1) = 0$, where $(u'_{i}, v'_{i}) = w(B, 1, i)$
        \item $acc = b_0 + b_1 \cdot 2 + b_2 \cdot 2^2 + b_3 \cdot 2^3 + b_4 \cdot 2^4 + b_5 \cdot 2^5 $
        \item $(x_1, y_1) = (u_0, v_0)$
        \item $(x_2, y_2) = (x_1, y_1) + (u_1, v_1)$ incomplete addition, where $x_1 \neq u_1$
    \end{itemize}
    \item For $i + z$, $z \in{1, ..., 41}$:
    \begin{itemize}
        \item $b_i \cdot (b_i - 1) = 0$, where $i \in\{0,.., 5\}$
        \item $\phi_1(b_0, b_1, b_2, u_0) = 0$, where $(u'_{i}, v'_{i}) = w(B, z \cdot 2, i)$
        \item $\phi_1(b_3, b_4, b_5, u_1) = 0$, where $(u'_{i}, v'_{i}) = w(B, z \cdot 2 + 1, i)$
        \item $\phi_2(b_0, b_1, b_2, v_0) = 0$, where $(u'_{i}, v'_{i}) = w(B, z \cdot 2, i)$
        \item $\phi_2(b_3, b_4, b_5, v_1) = 0$, where $(u'_{i}, v'_{i}) = w(B, z \cdot 2 + 1, i)$
        \item $acc = b_0 + b_1 \cdot 2 + b_2 \cdot 2^2 + b_3 \cdot 2^3 + b_4 \cdot 2^4 + b_5 \cdot 2^5 + acc_{prev} \cdot 2^6$
        \item $(x_1, y_1) = (u_0, v_0) + (x_2, y_2)_{prev}$  incomplete addition, where $u_0 \neq x_2$
        \item $(x_2, y_2) = (x_1, y_1) + (u_1, v_1)$ incomplete addition, where $x_1 \neq u_1$
    \end{itemize}
    \item For $i + 42$:
    \begin{itemize}
        \item $b_i \cdot (b_i - 1) = 0$, where $i \in\{0,.., 2\}$
        \item $\phi_1(b_0, b_1, b_2, u_0) = 0$, where $(u'_{i}, v'_{i}) = w(B, 84, i)$
        \item $\phi_2(b_0, b_1, b_2, v_0) = 0$, where $(u'_{i}, v'_{i}) = w(B, 84, i)$
        \item $b = b_0 + b_1 \cdot 2 + b_2 \cdot 2^2 + acc_{prev} \cdot 2^3$
        \item $(x_w, y_w) = (u_0, v_0) + (x_2, y_2)_{prev}$  complete addition from \href{https://zcash.github.io/orchard/design/circuit/gadgets/ecc/addition.html} {Orchard}
    \end{itemize}
\end{itemize}